expr_db_nat.v
@@ -1,3 +1,4 @@
+Require Import util List Arith.Peano_dec.
 Inductive expr : Type := 
   | var : nat -> expr 
   | lam : expr -> expr
@@ -7,6 +8,14 @@ Definition value (t : expr) : Prop := match t with
   | lam _ => True
   | _ => False
   end.
+
+Fixpoint fvs (e:expr) : list nat := match e with
+  | var v =>  v::nil
+  | lam b =>  map pred (remove eq_nat_dec 0 (fvs b))
+  | app m n => fvs m ++ fvs n
+  end.
+
+Definition closed (e:expr) := fvs e = nil.
 
 Notation " :λ N " := (lam N) (at level 20).
 Notation " M @ N " := (app M N) (at level 60). 
