cem_cbn_bisim.v
@@ -1,8 +1,19 @@
+Require Import Unicode.Utf8.
 Require Import bisim db List NaryFunctions.
 Require cem cbn expr expr_db_nat.
+Require Import CpdtTactics.
 
-(* Basic idea of proof: we use substitution equivalence relation : substituting
-all terms into the term from the heap, then converting to deBruijn indices *) 
+(*Well formed configurations can be collapsed into a closed deBruijn term*)
+Theorem well_formed_cbn_closed_db : ∀ c, cbn.well_formed c -> {e | expr_db_nat.closed e}.
+intros. destruct c. induction (expr.fvs t). destruct H. 
+induction h. destruct H. crush. assert (expr.closed t).
+unfold expr.closed. apply util.subset_nil2. assumption. apply dbf. split with
+(x:=t). assumption. destruct a. crush. 
+
+apply dbf.
+
+(* Relation idea: replace deBruijn variable with lookup location, which makes
+them equal *)
 
 Inductive state_rel : relation cem.configuration cbn.configuration := 
   | init : forall t e,
